src/cbor/pulse/raw/everparse/CBOR.Pulse.Raw.EverParse.Serialized.Rust.fsti
@@ -1,0 +1,26 @@
+module CBOR.Pulse.Raw.EverParse.Serialized.Rust
+open LowParse.Spec.Base
+open LowParse.Pulse.Base
+open Pulse.Lib.Pervasives
+open CBOR.Spec.Raw.Base
+open CBOR.Spec.Raw.EverParse
+open CBOR.Pulse.Raw.Match.Gen.Base
+
+module S = Pulse.Lib.Slice.Util
+module Trade = Pulse.Lib.Trade.Util
+module Match = CBOR.Pulse.Raw.Match
+
+val cbor_read
+  (input: S.slice byte)
+  (#pm: perm)
+  (#v: Ghost.erased raw_data_item)
+: stt (cbor_serialized_raw Match.cbor_string Match.cbor_serialized)
+  (requires
+    pts_to_serialized serialize_raw_data_item input #pm v
+  )
+  (ensures fun res ->
+      cbor_serialized_raw_match Match.cbor_match_string Match.cbor_match_serialized_array Match.cbor_match_serialized_map Match.cbor_match_serialized_tagged 1.0R res v **
+      Trade.trade
+        (cbor_serialized_raw_match Match.cbor_match_string Match.cbor_match_serialized_array Match.cbor_match_serialized_map Match.cbor_match_serialized_tagged 1.0R res v)
+        (pts_to_serialized serialize_raw_data_item input #pm v)
+  )
